

---

# P2 Chapter 1: Algebra Techniques

## Partial Fractions

# Partial Fractions

If the **denominator is a product of a linear terms**, it can be split into the sum of 'partial fractions', where **each denominator is a single linear term**.

$$\frac{6x - 2}{(x - 3)(x + 1)} \equiv \frac{A}{x - 3} + \frac{B}{x + 1}$$

**Notation reminder:**  $\equiv$  means 'equivalent/identical to', and indicates that both sides are equal for all values of  $x$ .

## Method 1: Substitution

$$6x - 2 \equiv A(x + 1) + B(x - 3)$$

Let  $x = -1$ :

$$-8 = -4B \rightarrow B = 2$$

Let  $x = 3$ :

$$16 = 4A \rightarrow A = 4$$

$$\therefore \frac{6x - 2}{(x - 3)(x + 1)} \equiv \frac{4}{x - 3} + \frac{2}{x + 1}$$

We don't like fractions, so multiply through by denominator of LHS. See note below.

Choose values of  $x$  that make one of brackets disappear.

When we multiply  $\frac{A}{x-3}$  by  $(x-3)(x+1)$ , multiplying initially by  $(x-3)$  cancels out the "over  $x-3$ ", but we still need to multiply by the  $(x+1)$ , giving  $A(x+1)$ . The textbook instead has an intermediate step of adding the fractions on the RHS first, but I feel this is unnecessary.

## Method 2: Comparing Coefficients

$$6x - 2 \equiv A(x + 1) + B(x - 3)$$

Comparing coefficients of  $x$  terms:

$$6 = A + B$$

Comparing constant terms:

$$-2 = A - 3B$$

Solving simultaneously:

$$A = 4, \quad B = 2$$

$$\therefore \frac{6x - 2}{(x - 3)(x + 1)} \equiv \frac{4}{x - 3} + \frac{2}{x + 1}$$

If two sides are identical,  $x$  terms must match, constant terms must match and so on, e.g. if  $3x + 4 \equiv ax + b$  Then  $a = 3$  and  $b = 4$ , whereas this is not necessarily true for a normal equality.

# Further Example

Given that  $\frac{6x^2+5x-2}{x(x-1)(2x+1)} \equiv \frac{A}{x} + \frac{B}{x-1} + \frac{C}{2x+1}$ , find the values of the constants  $A, B, C$ .

$$6x^2 + 5x - 2 \equiv A(x-1)(2x+1) + Bx(2x+1) + Cx(x-1)$$

Let  $x = 1$ :

$$9 = 3B \quad \rightarrow \quad B = 3$$

Let  $x = -\frac{1}{2}$ :

$$-3 = \frac{3}{4}C \quad \rightarrow \quad C = -4$$

Let  $x = 0$ :

$$-2 = -A \quad \rightarrow \quad A = 2$$

$$\therefore \frac{6x^2 + 5x - 2}{x(x-1)(2x+1)} \equiv \frac{2}{x} + \frac{3}{x-1} - \frac{4}{2x+1}$$

# Test Your Understanding

C4 June 2005 Q3a

Express  $\frac{5x+3}{(2x-3)(x+2)}$  in partial fractions.

**(3)**

?

# Test Your Understanding

C4 June 2005 Q3a

Express  $\frac{5x+3}{(2x-3)(x+2)}$  in partial fractions.

**(3)**

(a) 
$$\frac{5x+3}{(2x-3)(x+2)} = \frac{A}{2x-3} + \frac{B}{x+2}$$

$$5x+3 = A(x+2) + B(2x-3)$$

Substituting  $x = -2$  or  $x = \frac{3}{2}$  and obtaining  $A$  or  $B$ ; or equating coefficients and solving a pair of simultaneous equations to obtain  $A$  or  $B$ .

$$A = 3, B = 1$$

If the cover-up rule is used, give M1 A1 for the first of  $A$  or  $B$  found, A1 for the second.

M1

A1, A1

**(3)**

# Exercise 1.3

Pearson Pure Mathematics Year 2/AS

Page 2

---

# Homework Exercise

1 Express the following as partial fractions:

a  $\frac{6x - 2}{(x - 2)(x + 3)}$

b  $\frac{2x + 11}{(x + 1)(x + 4)}$

c  $\frac{-7x - 12}{2x(x - 4)}$

d  $\frac{2x - 13}{(2x + 1)(x - 3)}$

e  $\frac{6x + 6}{x^2 - 9}$

**Hint** First factorise the denominator.

f  $\frac{7 - 3x}{x^2 - 3x - 4}$

g  $\frac{8 - x}{x^2 + 4x}$

h  $\frac{2x - 14}{x^2 + 2x - 15}$

2 Show that  $\frac{-2x - 5}{(4 + x)(2 - x)}$  can be written in the form  $\frac{A}{4 + x} + \frac{B}{2 - x}$  where  $A$  and  $B$  are constants to be found.

(3 marks)

3 The expression  $\frac{A}{(x - 4)(x + 8)}$  can be written in partial fractions as  $\frac{2}{x - 4} + \frac{B}{x + 8}$   
Find the values of the constants  $A$  and  $B$ .

4  $h(x) = \frac{2x^2 - 12x - 26}{(x + 1)(x - 2)(x + 5)}, x > 2$

Given that  $h(x)$  can be expressed in the form  $\frac{A}{x + 1} + \frac{B}{x - 2} + \frac{C}{x + 5}$ , find the values of  $A$ ,  $B$  and  $C$ .

(4 marks)

# Homework Exercise

- E** 5 Given that, for  $x < -1$ ,  $\frac{-10x^2 - 8x + 2}{x(2x + 1)(3x - 2)} \equiv \frac{D}{x} + \frac{E}{2x + 1} + \frac{F}{3x - 2}$ , where  $D$ ,  $E$  and  $F$  are constants. Find the values of  $D$ ,  $E$  and  $F$ . **(4 marks)**

6 Express the following as partial fractions:

**a**  $\frac{2x^2 - 12x - 26}{(x + 1)(x - 2)(x + 5)}$

**b**  $\frac{-10x^2 - 8x + 2}{x(2x + 1)(3x - 2)}$

**c**  $\frac{-5x^2 - 19x - 32}{(x + 1)(x + 2)(x - 5)}$

**P** 7 Express the following as partial fractions:

**a**  $\frac{6x^2 + 7x - 3}{x^3 - x}$

**b**  $\frac{8x + 9}{10x^2 + 3x - 4}$

**Hint**

First factorise the denominator.

## Challenge

Express  $\frac{5x^2 - 15x - 8}{x^3 - 4x^2 + x + 6}$  as a sum of fractions with linear denominators.



# Homework Answers

1 a  $\frac{4}{x+3} + \frac{2}{x-2}$

c  $\frac{3}{2x} - \frac{5}{x-4}$

e  $\frac{2}{x+3} + \frac{4}{x-3}$

g  $\frac{2}{x} - \frac{3}{x+4}$

2  $A = \frac{1}{2}, B = -\frac{3}{2}$

3  $A = 24, B = -2$

4  $A = 1, B = -2, C = 3$

5  $D = -1, E = 2, F = -5$

6  $\frac{3}{x+1} - \frac{2}{x+2} - \frac{6}{x-5}$

7 a  $\frac{3}{x} - \frac{2}{x+1} + \frac{5}{x-1}$

b  $\frac{-1}{5x+4} + \frac{2}{2x-1}$

b  $\frac{3}{x+1} - \frac{1}{x+4}$

d  $\frac{4}{2x+1} - \frac{1}{x-3}$

f  $-\frac{2}{x+1} - \frac{1}{x-4}$

h  $\frac{3}{x+5} - \frac{1}{x-3}$

## Challenge

$$\frac{6}{x-2} + \frac{1}{x+1} - \frac{2}{x-3}$$